Hnr_Case_Rules.thy
@@ -1,9 +1,9 @@
 theory Hnr_Case_Rules
-  imports Hnr_Base Keep_Drop Merge
+  imports Hnr_Base Keep_Drop Norm Merge
 begin
 
 (* TODO:
-  - Is it possible to generalize that it works with every case distinction
+  - Is it possible to generalize that it works with every case distinction?
   - Find a way to make case distinctions also work if they are on a refined type/ a type that
     contains a refined type
 *)
@@ -13,14 +13,14 @@ lemma hnr_bind [hnr_rule]:
     "hnr \<Gamma> vi \<Gamma>\<^sub>1 v" 
     "\<And>x xi. hnr (\<Gamma>\<^sub>1 x xi) (fi xi) (\<Gamma>' x xi) (f x)"
     "\<And>x xi r ri. Keep_Drop (\<Gamma>' x xi r ri) (\<Gamma>'' r ri) (\<Gamma>\<^sub>1' x xi r ri)"
-    "\<And>r ri. Simp (\<Gamma>'' r ri) (\<Gamma>''' r ri)" 
+    "\<And>r ri. Norm (\<Gamma>'' r ri) (\<Gamma>''' r ri)" 
   shows 
     "hnr \<Gamma> (do { x \<leftarrow> vi; fi x }) \<Gamma>''' (do { x \<leftarrow> v; f x })"
   supply[sep_heap_rules] = assms(1, 2)[THEN hnrD]
   apply(rule hnrI)
   apply(sep_auto split: option.splits Option.bind_splits)
   apply(sep_drule r: assms(3)[unfolded Keep_Drop_def])
-  apply(sep_drule r: assms(4)[unfolded Simp_def])
+  apply(sep_drule r: assms(4)[unfolded Norm_def])
   by sep_auto
 
 lemma hnr_if [hnr_rule]: 
@@ -55,7 +55,7 @@ method hnr_cases_solve_case uses case_hnr ent_disjI =
     rule cons_post_rule,
     rule fi_rule,
     rule case_hnr[THEN hnrD],
-    (sep_auto simp: Keep_Drop_def Simp_def id_rel_def)+,
+    (sep_auto simp: Keep_Drop_def Norm_def id_rel_def)+,
     meson ent_disjI ent_refl_true ent_trans ent_true_drop(1)
 
 lemma hnr_case_tuple [hnr_rule]:
@@ -67,7 +67,7 @@ lemma hnr_case_tuple [hnr_rule]:
         (\<Gamma>\<^sub>a a ai b bi)
         (c a b)"
     "\<And>a ai b bi ri r. Keep_Drop (\<Gamma>\<^sub>a a ai b bi r ri) (\<Gamma>\<^sub>a' r ri) (\<Gamma>Drop a ai b bi r ri)"
-    "\<And>r ri. Simp (\<Gamma>\<^sub>a' r ri) (\<Gamma>\<^sub>a'' r ri)"
+    "\<And>r ri. Norm (\<Gamma>\<^sub>a' r ri) (\<Gamma>\<^sub>a'' r ri)"
   shows
     "hnr (\<Gamma> * id_assn x xi) (case xi of (ai, bi) \<Rightarrow> ci ai bi) \<Gamma>\<^sub>a'' (case x of (a, b) \<Rightarrow> c a b)"
   apply(hnr_cases_prepare splits: prod.splits)
@@ -79,16 +79,19 @@ lemma hnr_case_sum [hnr_rule]:
   assumes 
     "\<And>s' si'. hnr (\<Gamma> * id_assn s si * id_assn s' si') (cli si') (\<Gamma>\<^sub>a s' si') (cl s')"
     "\<And>l' li' ri r. Keep_Drop (\<Gamma>\<^sub>a l' li' r ri) (\<Gamma>\<^sub>a' r ri) (Drop\<^sub>a l' li' r ri)"
-    "\<And>r ri. Simp (\<Gamma>\<^sub>a' r ri) (\<Gamma>\<^sub>a'' r ri)" 
+    "\<And>r ri. Norm (\<Gamma>\<^sub>a' r ri) (\<Gamma>\<^sub>a'' r ri)" 
 
     "\<And>s' si'. hnr (\<Gamma> * id_assn s si * id_assn s' si') (cri si') (\<Gamma>\<^sub>b s' si') (cr s')"
     "\<And>r' ri' ri r. Keep_Drop (\<Gamma>\<^sub>b r' ri' r ri) (\<Gamma>\<^sub>b' r ri) (Drop\<^sub>b r' ri' r ri)"
-    "\<And>r ri. Simp (\<Gamma>\<^sub>b' r ri) (\<Gamma>\<^sub>b'' r ri)" 
+    "\<And>r ri. Norm (\<Gamma>\<^sub>b' r ri) (\<Gamma>\<^sub>b'' r ri)" 
 
     "\<And>r ri. Merge (\<Gamma>\<^sub>a'' r ri) (\<Gamma>\<^sub>b'' r ri) (\<Gamma>\<^sub>c r ri)"
   shows
-    "hnr (\<Gamma> * id_assn s si)
-         (case si of Inl l \<Rightarrow> cli l | Inr r \<Rightarrow> cri r) \<Gamma>\<^sub>c (case s of Inl l \<Rightarrow> cl l | Inr r \<Rightarrow> cr r)"
+    "hnr 
+      (\<Gamma> * id_assn s si)
+      (case si of Inl l \<Rightarrow> cli l | Inr r \<Rightarrow> cri r)
+       \<Gamma>\<^sub>c 
+      (case s of Inl l \<Rightarrow> cl l | Inr r \<Rightarrow> cr r)"
   using assms(7)
   apply -
   apply(hnr_cases_prepare splits: sum.splits)
@@ -106,7 +109,7 @@ lemma hnr_case_nat[hnr_rule]:
     "hnr (\<Gamma> * id_assn n ni) ci0 \<Gamma>\<^sub>a c0"
     "\<And>n' ni'. hnr (\<Gamma> * id_assn n ni * id_assn n' ni') (ci ni') (\<Gamma>\<^sub>b n' ni') (c n')"
     "\<And>n ni ri r. Keep_Drop (\<Gamma>\<^sub>b n ni r ri) (\<Gamma>\<^sub>b' r ri) (Drop n ni r ri)"
-    "\<And>r ri. Simp (\<Gamma>\<^sub>b' r ri) (\<Gamma>\<^sub>b'' r ri)" 
+    "\<And>r ri. Norm (\<Gamma>\<^sub>b' r ri) (\<Gamma>\<^sub>b'' r ri)" 
     "\<And>r ri. Merge (\<Gamma>\<^sub>a r ri) (\<Gamma>\<^sub>b'' r ri) (\<Gamma>\<^sub>c r ri)"
   shows
     "hnr 
@@ -134,7 +137,7 @@ lemma hnr_case_list [hnr_rule]:
         (\<Gamma>\<^sub>b x' xi' xs' xsi')
         (c x' xs')"
     "\<And>x xi xs xsi ri r. Keep_Drop (\<Gamma>\<^sub>b x xi xs xsi r ri) (\<Gamma>\<^sub>b' r ri) (Drop x xi xs xsi r ri)"
-    "\<And>r ri. Simp (\<Gamma>\<^sub>b' r ri) (\<Gamma>\<^sub>b'' r ri)"
+    "\<And>r ri. Norm (\<Gamma>\<^sub>b' r ri) (\<Gamma>\<^sub>b'' r ri)"
     "\<And>r ri. Merge (\<Gamma>\<^sub>a r ri) (\<Gamma>\<^sub>b'' r ri) (\<Gamma>\<^sub>c r ri)"
   shows
     "hnr 
