Keep_Drop.thy
@@ -2,53 +2,42 @@ theory Keep_Drop
   imports Base
 begin
 
-lemma keep_drop_1:
+definition Keep_Drop where 
+  "Keep_Drop \<Gamma> K D \<equiv> \<Gamma> \<Longrightarrow>\<^sub>A K * D"
+
+lemma init:
+  assumes
+    "\<Gamma> \<Longrightarrow>\<^sub>A K * D"
+  shows
+    "Keep_Drop \<Gamma> K D"
+  unfolding Keep_Drop_def
+  using assms by simp
+
+lemma split:
   assumes
     "\<Gamma>\<^sub>1 \<Longrightarrow>\<^sub>A K\<^sub>1 * D\<^sub>1"
     "\<Gamma>\<^sub>2 \<Longrightarrow>\<^sub>A K\<^sub>2 * D\<^sub>2"
   shows 
-    "\<Gamma>\<^sub>1 * \<Gamma>\<^sub>2 \<Longrightarrow>\<^sub>A (K\<^sub>1 * K\<^sub>2) * (D\<^sub>1 * D\<^sub>2)"
+    "\<Gamma>\<^sub>1 * \<Gamma>\<^sub>2 \<Longrightarrow>\<^sub>A (K\<^sub>1 * K\<^sub>2) * (D\<^sub>1 * D\<^sub>2)" 
   apply(sep_drule r: assms(1))
   apply(sep_drule r: assms(2))
   by sep_auto
 
-lemma keep_drop_2: 
+lemma keep: 
   assumes
-    "A \<Longrightarrow>\<^sub>A A'"
+    "\<Gamma> \<Longrightarrow>\<^sub>A \<Gamma>'"
   shows
-    "A \<Longrightarrow>\<^sub>A A' * emp"
+    "\<Gamma> \<Longrightarrow>\<^sub>A \<Gamma>' * emp"
   using assms
   by sep_auto
 
-lemma keep_drop_3: "A \<Longrightarrow>\<^sub>A emp * A"
+lemma drop: "\<Gamma> \<Longrightarrow>\<^sub>A emp * \<Gamma>"
   by simp
 
-lemmas keep_drop_step = keep_drop_1 keep_drop_2 keep_drop_3
-
-definition Keep_Drop where "Keep_Drop \<Gamma> K D \<equiv> \<Gamma> \<Longrightarrow>\<^sub>A K * D"
-
-definition Simp where
-  "Simp a b \<equiv> a \<Longrightarrow>\<^sub>A b"
-
-lemma keep_drop_init:
-  assumes
-    "\<Gamma>  \<Longrightarrow>\<^sub>A K * D"
-  shows
-    "Keep_Drop \<Gamma> K D"
-  unfolding Keep_Drop_def
-  using assms(1) ent_star_mono ent_trans by blast
-
-lemma keep_drop_simpI: "a \<Longrightarrow>\<^sub>A b \<Longrightarrow> Simp a b"
-  unfolding Simp_def
-  by simp
-
-method keep_drop_simp = 
-  rule keep_drop_simpI, (simp only: star_aci)?; rule ent_refl
-
-method keep_drop_step methods keep_atom = 
-  rule keep_drop_1 | (rule keep_drop_2, keep_atom) | rule keep_drop_3
+method keep_drop_step methods keep_atom =
+  rule split | (rule keep, keep_atom) | rule drop
 
 method keep_drop methods keep_atom = 
-  rule keep_drop_init, ((keep_drop_step keep_atom)+; fail)
+  rule init, ((keep_drop_step keep_atom)+; fail)
 
 end
