Norm.thy
@@ -1,0 +1,15 @@
+theory Norm
+  imports Base
+begin
+
+definition Norm where
+  "Norm \<Gamma> \<Gamma>' \<equiv> \<Gamma> \<Longrightarrow>\<^sub>A \<Gamma>'"
+
+lemma normI: "\<Gamma> \<Longrightarrow>\<^sub>A \<Gamma>' \<Longrightarrow> Norm \<Gamma> \<Gamma>'"
+  unfolding Norm_def
+  by simp
+
+method normalize =
+  rule normI, (simp only: star_aci)?; rule ent_refl
+             
+end
